#C27-4 

#ProofDeferred #GotIt 

This [[derivation]] follows trivially from the definition of [[work]] and [[Ã˜rsted-Laplace-Thomson law]]: 

$F_\text{B} = q\vec{v}\times\vec{B}$, and $W = \vec{F} \cdot \vec{d}$ so over a duration $\partial t$$ $$\vec{d} = q\vec{v}\partial t$$
$$W = (q\vec{v}\times\vec{B})\cdot q\vec{v}\partial t = q\vec{v}\partial t\cdot(q\vec{v}\times\vec{B})$$
since $q\vec{v} \ || \ q\vec{v}\partial t$, and $q\vec{v}\partial t \perp (q\vec{v}\times\vec{B})$, $$q\vec{v}\partial t\cdot (q\vec{v}\times\vec{B})=|qv\partial t|||qvB|\sin{\phi}|\cos(90^\circ) = 0$$
or following from the properties of the scalar triple product,
$$W = (q\vec{v}\times\vec{B})\cdot q\vec{v}\partial t = q\vec{v}\partial t\cdot(q\vec{v}\times\vec{B}) = \vec{B}\cdot(q\vec{v}\partial t\times q\vec{v}) = \vec{B}\cdot\vec{0}=0$$
